Update

googology.v
@@ -14,8 +14,8 @@ Definition ind : forall (P : Type), P -> (P -> P) -> nat -> P :=
    end
 .
 
-Definition comp : forall (A B C : Type), (B -> C) -> (A -> B) -> A -> C :=
- fun (A B C : Type) (f : B -> C) (g : A -> B) (x : A) => f (g x)
+Definition comp : forall (A : Type), (A -> A) -> (nat -> A) -> nat -> A :=
+ fun (A : Type) (f : A -> A) (g : nat -> A) (x : nat) => f (g x)
 .
 
 Definition to : Type := nat.
@@ -38,7 +38,7 @@ Definition t0 : Type := ts t.
 
 Definition o0 : t0 := ind t o s.
 
-Definition s0 : t0 -> t0 := comp nat t t s.
+Definition s0 : t0 -> t0 := comp t s.
 
 Definition f01 : t0 := o0.
 
@@ -50,7 +50,7 @@ Definition t00 : Type := ts t0.
 
 Definition o00 : t00 := ind t0 o0 s0.
 
-Definition s00 : t00 -> t00 := comp nat t0 t0 s0.
+Definition s00 : t00 -> t00 := comp t0 s0.
 
 Definition f0101 : t00 := o00.
 
@@ -58,73 +58,52 @@ Definition f01010 : t00 := s00 f0101.
 
 Definition f010100 : t00 := s00 f01010.
 
-Definition t000 : Type := ts t00.
+Definition t01 : nat -> Type := ind Type to ts.
 
-Definition o000 : t000 := ind t00 o00 s00.
+Definition o01 : forall m, t01 m.
+Proof.
+ refine (fix o01 m := _).
+ refine (match m as m' return t01 m' with O => _ | S mp => _ end).
+ -
+  refine o.
+ -
+  refine (ind (t01 mp) (o01 mp) _).
+  refine ((_ : forall m, t01 m -> t01 m) mp).
+  refine (fix scheme n := _).
+  refine (match n as n' return t01 n' -> t01 n' with O => _ | S np => _ end).
+  +
+   refine s.
+  +
+   refine (comp (t01 np) (scheme np)).
+Defined.
 
-Definition s000 : t000 -> t000 := comp nat t00 t00 s00.
-
-Definition f010101 : t000 := o000.
-
-Definition f0101010 : t000 := s000 f010101.
-
-Definition f01010100 : t000 := s000 f0101010.
-
-Definition indD
- :
-  forall (P : nat -> Type), P O -> (forall (x : nat), P x -> P (S x)) -> forall (x : nat), P x
- :=
-  nat_rect
-.
-
-Definition compD
- :
-  forall (A : Type) (B : A -> Type) (C : A -> Type),
-   (forall (x : A), B x -> C x) -> (forall (x : A), B x) -> forall (x : A), C x
- :=
-  fun
-   (A : Type)
-   (B : A -> Type)
-   (C : A -> Type)
-   (f : forall (x : A), B x -> C x)
-   (g : forall (x : A), B x)
-   (x : A)
-  => f x (g x)
-.
-
-Definition to0 : nat -> Type := ind Type to ts.
-
-Definition ts0 : (nat -> Type) -> nat -> Type := comp nat Type Type ts.
-
-Definition t01 : nat -> Type := to0.
-
-Definition s01 : forall (x : nat), to0 x -> to0 x :=
- indD
-  (fun x => to0 x -> to0 x)
-  s
-  (fun (xp : nat) => comp nat (to0 xp) (to0 xp))
-.
-
-Definition o01 : forall (x : nat), to0 x :=
- indD
-  (fun x => to0 x)
-  o
-  (fun (xp : nat) (go : to0 xp) => ind (to0 xp) go (s01 xp))
-.
+Definition s01 : (forall m, t01 m) -> (forall m, t01 m).
+Proof.
+ refine (fun f m => _).
+ refine (_ (f m)).
+ refine ((_ : forall n, t01 n -> t01 n) m).
+ refine (fix scheme n := _).
+ refine (match n as n' return t01 n' -> t01 n' with O => _ | S np => _ end).
+ -
+  refine s.
+ -
+  refine (comp (t01 np) (scheme np)).
+Defined.
 
 Definition f011 : forall (x : nat), t01 x := o01.
 
-Definition f0110 : forall (x : nat), t01 x := compD nat t01 t01 s01 f011.
+Definition f0110 : forall (x : nat), t01 x := s01 f011.
 
-Definition f01100 : forall (x : nat), t01 x := compD nat t01 t01 s01 f0110.
+Definition f01100 : forall (x : nat), t01 x := s01 f0110.
 
-Definition t010 : nat -> Type := ts0 t01.
+Definition t010 : Type := ts (forall m, t01 m).
+
+Definition o010 : t010 :=
+ indD t010 s (fun (xp : nat) (go : t010 xp) => ind (t010 xp) go (s010 xp)).
 
 Definition s010 : forall (x : nat), t010 x -> t010 x :=
  fun (x : nat) => comp nat (t01 x) (t01 x) (s01 x).
 
-Definition o010 : forall (x : nat), t010 x :=
- indD t010 s (fun (xp : nat) (go : t010 xp) => ind (t010 xp) go (s010 xp)).
 
 Definition f01101 : forall (x : nat), t010 x := o010.
 
